src/BinEncoders/Env/Examples/DnsOpt.v
@@ -38,6 +38,155 @@ Section DnsPacket.
   Variable cacheAddDNPointer : CacheAdd cache (string * pointerT).
   Variable cacheGetDNPointer : CacheGet cache string pointerT.
   Variable cachePeekDNPointer : CachePeek cache pointerT.
+  Variable IndependentCaches :
+    forall env p (b : nat),
+      getD (addD env b) p = getD env p.
+  Variable GetCacheAdd_1 :
+    forall env (p : pointerT) (domain : string),
+      getD (addD env (domain, p)) p = Some domain.
+  Variable GetCacheAdd_2 :
+    forall env (p p' : pointerT) (domain : string),
+      p <> p' -> getD (addD env (domain, p')) p = getD env p.
+
+  Definition GoodCache (env : CacheDecode) :=
+    forall domain p,
+      getD env p = Some domain
+      -> ValidDomainName domain
+         /\ (String.length domain > 0)%nat.
+  
+  Lemma cacheIndependent_add
+    : forall (b : nat) (cd : CacheDecode),
+      GoodCache cd -> GoodCache (addD cd b).
+  Proof.
+    unfold GoodCache; intros.
+    rewrite IndependentCaches in *; eauto.
+  Qed.
+
+  Lemma cacheIndependent_add_2
+    : forall cd p (b : nat) domain,
+      GoodCache cd
+      -> getD (addD cd b) p = Some domain
+      -> forall pre label post : string,
+          domain = (pre ++ label ++ post)%string ->
+          ValidLabel label -> (String.length label <= 63)%nat.
+  Proof.
+    unfold GoodCache; intros.
+    rewrite IndependentCaches in *; eapply H; eauto.
+  Qed.
+  
+  Lemma cacheIndependent_add_3
+    : forall cd p (b : nat) domain,
+      GoodCache cd
+      -> getD (addD cd b) p = Some domain
+      -> ValidDomainName domain.
+  Proof.
+    unfold GoodCache; intros.
+    rewrite IndependentCaches in *; eapply H; eauto.
+  Qed.
+  
+  Lemma cacheIndependent_add_4
+    : forall cd p (b : nat) domain,
+      GoodCache cd
+      -> getD (addD cd b) p = Some domain
+      -> gt (String.length domain) 0.
+  Proof.
+    unfold GoodCache; intros.
+    rewrite IndependentCaches in *; eapply H; eauto.
+  Qed.
+  
+  Lemma cacheIndependent_add_5
+    : forall cd p domain,
+      GoodCache cd
+      -> getD cd p = Some domain
+      -> ValidDomainName domain.
+  Proof.
+    unfold GoodCache; intros.
+    eapply H; eauto.
+  Qed.
+  
+  Lemma cacheIndependent_add_6
+    : forall cd p domain,
+      GoodCache cd
+      -> getD cd p = Some domain
+      -> gt (String.length domain) 0.
+  Proof.
+    unfold GoodCache; intros.
+    eapply H; eauto.
+  Qed.
+  
+  Lemma cacheIndependent_add_7
+    : forall cd p domain,
+      GoodCache cd
+      -> getD cd p = Some domain
+      -> forall pre label post : string,
+          domain = (pre ++ label ++ post)%string ->
+          ValidLabel label -> (String.length label <= 63)%nat.
+  Proof.
+    unfold GoodCache; intros.
+    eapply H; eauto.
+  Qed.
+
+  Lemma ptr_eq_dec :
+    forall (p p' : pointerT),
+      {p = p'} + {p <> p'}.
+  Proof.
+    decide equality.
+    apply weq.
+    destruct a; destruct s; simpl in *.
+    destruct (weq x x0); subst.
+    left; apply ptr_eq; reflexivity.
+    right; unfold not; intros; apply n.
+    congruence.
+  Qed.
+    
+  Lemma cacheIndependent_add_8
+    : forall cd p p0 domain domain',
+      GoodCache cd
+      -> ValidDomainName domain' /\ (String.length domain' > 0)%nat
+      -> getD (addD cd (domain', p0)) p = Some domain
+      -> forall pre label post : string,
+          domain = (pre ++ label ++ post)%string ->
+          ValidLabel label -> (String.length label <= 63)%nat.
+  Proof.
+    unfold GoodCache; intros.
+    destruct (ptr_eq_dec p p0); subst.
+    - rewrite GetCacheAdd_1 in H1; injections.
+      destruct H0.
+      eapply H0; eauto.
+    - rewrite GetCacheAdd_2 in H1 by eauto.
+      eapply H; eauto.
+  Qed.
+  
+  Lemma cacheIndependent_add_9
+      : forall cd p p0 domain domain',
+        GoodCache cd
+        -> ValidDomainName domain' /\ (String.length domain' > 0)%nat
+        -> getD (addD cd (domain', p0)) p = Some domain
+        -> ValidDomainName domain.
+  Proof.
+    unfold GoodCache; intros.
+    destruct (ptr_eq_dec p p0); subst.
+    - rewrite GetCacheAdd_1 in H1; injections.
+      destruct H0.
+      eapply H0; eauto.
+    - rewrite GetCacheAdd_2 in H1 by eauto.
+      eapply H; eauto.
+  Qed.
+
+  Lemma cacheIndependent_add_10
+    : forall cd p p0 domain domain',
+      GoodCache cd
+      -> ValidDomainName domain' /\ (String.length domain' > 0)%nat
+      -> getD (addD cd (domain', p0)) p = Some domain
+      -> gt (String.length domain) 0.
+  Proof.
+    unfold GoodCache; intros.
+    destruct (ptr_eq_dec p p0); subst.
+    - rewrite GetCacheAdd_1 in H1; injections.
+      destruct H0; apply H1.
+    - rewrite GetCacheAdd_2 in H1 by eauto.
+      eapply H; eauto.
+  Qed.    
 
   Variable QType_Ws : t (word 16) 17.
   Variable QType_Ws_OK : NoDupVector QType_Ws.
@@ -175,12 +324,26 @@ Section DnsPacket.
     f_equal; eauto.
   Qed.
 
+  Lemma decides_firstn_app {A}
+    : forall (l1 l2 : list A),
+      decides true (firstn (|l1 |) (l1 ++ l2) = l1).
+  Proof.
+    apply firstn_app.
+  Qed.
+
   Lemma firstn_self {A}
     : forall (l1 : list A),
       firstn (|l1 |) l1 = l1.
   Proof.
     induction l1; intros; simpl; eauto.
     f_equal; eauto.
+  Qed.
+
+  Lemma decides_firstn_self {A}
+    : forall (l1 : list A),
+      decides true (firstn (|l1 |) l1 = l1).
+  Proof.
+    intros; apply firstn_self.
   Qed.
 
   Lemma skipn_app {A}
@@ -190,6 +353,13 @@ Section DnsPacket.
     induction l1; intros; simpl; eauto.
   Qed.
 
+  Lemma decides_skipn_app {A}
+    : forall (l1 l2 : list A),
+      decides true (skipn (|l1|) (l1 ++ l2) = l2).
+  Proof.
+    apply skipn_app.
+  Qed.
+
   Lemma firstn_skipn_app {A}
     : forall (l1 l2 l3 : list A),
       firstn (|l3|) (skipn (|l1| + |l2|) (l1 ++ l2 ++ l3)) = l3.
@@ -197,6 +367,13 @@ Section DnsPacket.
     simpl; intros.
     rewrite <- app_length, List.app_assoc, skipn_app.
     apply firstn_self.
+  Qed.
+
+  Lemma decides_firstn_skipn_app {A}
+    : forall (l1 l2 l3 : list A),
+      decides true (firstn (|l3|) (skipn (|l1| + |l2|) (l1 ++ l2 ++ l3)) = l3).
+  Proof.
+    intros; apply firstn_skipn_app.
   Qed.
 
   Lemma firstn_skipn_self' {A}
@@ -220,7 +397,25 @@ Section DnsPacket.
     intros; f_equal; eauto.
   Qed.
 
-    Lemma firstn_skipn_self {A}
+  Lemma firstn_skipn_self'' {A}
+    : forall (n m o : nat) (l : list A),
+      length l = n + (m + o)
+      ->
+      decides true ((firstn n l ++ firstn m (skipn n l) ++ firstn o (skipn (n + m) l))%list =
+                    l).
+  Proof.
+    intros; eapply firstn_skipn_self'.
+    omega.
+  Qed.
+
+  Lemma word_eq_self 
+    : forall (w : word 1),
+      decides true (WS (whd w) WO = w).
+  Proof.
+    simpl; intros; shatter_word w; reflexivity.
+  Qed.
+
+  Lemma firstn_skipn_self {A}
       : forall (n m o : nat) (l l1 l2 l3 : list A),
       (l1 ++ l2 ++ l3)%list = l ->
       (|l1|) = n ->
@@ -397,11 +592,55 @@ Proof.
   eapply NPeano.Nat.min_lt_iff; eauto.
 Qed.
 
-Hint Resolve validDomainName_proj1_OK : decide_data_invariant_db.
-Hint Resolve validDomainName_proj2_OK : decide_data_invariant_db.
-Hint Resolve firstn_lt_decides : decide_data_invariant_db.
+  Lemma whd_word_1_refl' :
+    forall (b : word 1),
+      decides true (WS (whd b) WO = b).
+  Proof.
+    intros; destruct (shatter_word_S b) as [? [? ?] ]; subst.
+    rewrite (shatter_word_0 x0); reflexivity.
+  Qed.
 
-Instance : DecideableEnsembles.Query_eq () :=
+  Lemma decides_length_firstn_skipn_app {A}
+    : forall (n m o : nat) (l : list A),
+      length l = n + (m + o)
+      -> decides true ((|firstn m (skipn n l) |) = m).
+  Proof.
+    setoid_rewrite plus_assoc'.
+    eapply length_firstn_skipn_app.
+  Qed.
+
+  Lemma decides_length_firstn_skipn_app' {A}
+    : forall (n m o : nat) (l : list A),
+      length l = n + (m + o)
+      -> decides true ((|firstn o (skipn (n + m) l) |) = o).
+  Proof.
+    setoid_rewrite plus_assoc'. 
+    apply length_firstn_skipn_app'.
+  Qed.
+
+  Lemma decides_length_firstn_skipn_app'' {A}
+    : forall (n m o : nat) (l : list A),
+      length l = n + (m + o)
+      -> decides true ((|firstn n l |) = n).
+  Proof.
+    setoid_rewrite plus_assoc'. 
+    apply length_firstn_skipn_app''.
+  Qed.
+  
+  Hint Resolve whd_word_1_refl' : decide_data_invariant_db.
+  Hint Resolve decides_length_firstn_skipn_app'' : decide_data_invariant_db.
+  Hint Resolve decides_length_firstn_skipn_app' : decide_data_invariant_db.
+  Hint Resolve decides_length_firstn_skipn_app : decide_data_invariant_db.
+  Hint Resolve validDomainName_proj1_OK : decide_data_invariant_db.
+  Hint Resolve validDomainName_proj2_OK : decide_data_invariant_db.
+  Hint Resolve firstn_lt_decides : decide_data_invariant_db.
+  Hint Resolve firstn_skipn_self'' : decide_data_invariant_db.
+  Hint Resolve decides_firstn_app : decide_data_invariant_db.
+  Hint Resolve decides_firstn_self : decide_data_invariant_db.
+  Hint Resolve decides_skipn_app : decide_data_invariant_db.
+  Hint Resolve decides_firstn_skipn_app : decide_data_invariant_db.
+  
+  Instance : DecideableEnsembles.Query_eq () :=
   {| A_eq_dec a a' := match a, a' with (), () => left (eq_refl _) end |}.
 
 Definition resourceRecord_OK (rr : resourceRecord) :=
@@ -455,92 +694,6 @@ Definition DNS_Packet_OK (data : packet) :=
   /\ forall (rr : resourceRecord),
       In rr (data!"answers" ++ data!"additional" ++ data!"authority")
       -> resourceRecord_OK rr.
-
-    Definition GoodCache (env : CacheDecode) :=
-                     forall domain p,
-                     getD env p = Some domain
-                     -> ValidDomainName domain
-                        /\ (String.length domain > 0)%nat.
-
-    Lemma foo : forall (b : nat) (cd : CacheDecode), GoodCache cd -> GoodCache (addD cd b).
-    Admitted.
-
-    Lemma foo2
-      : forall cd p (b : nat) domain,
-        GoodCache cd
-        -> getD (addD cd b) p = Some domain
-        -> forall pre label post : string,
-            domain = (pre ++ label ++ post)%string ->
-            ValidLabel label -> (String.length label <= 63)%nat.
-    Admitted.
-
-    Lemma foo3
-      : forall cd p (b : nat) domain,
-        GoodCache cd
-        -> getD (addD cd b) p = Some domain
-        -> ValidDomainName domain.
-    Admitted.
-
-    Lemma foo4
-      : forall cd p (b : nat) domain,
-        GoodCache cd
-        -> getD (addD cd b) p = Some domain
-        -> gt (String.length domain) 0.
-    Admitted.
-
-    Lemma foo5
-      : forall cd p domain,
-        GoodCache cd
-        -> getD cd p = Some domain
-        -> ValidDomainName domain.
-    Admitted.
-
-    Lemma foo6
-      : forall cd p domain,
-        GoodCache cd
-        -> getD cd p = Some domain
-        -> gt (String.length domain) 0.
-    Admitted.
-
-    Lemma foo7
-      : forall cd p domain,
-        GoodCache cd
-        -> getD cd p = Some domain
-        -> forall pre label post : string,
-            domain = (pre ++ label ++ post)%string ->
-            ValidLabel label -> (String.length label <= 63)%nat.
-    Admitted.
-
-    Lemma foo8
-      : forall cd p p0 domain domain',
-        GoodCache cd
-        -> ValidDomainName domain' /\ (String.length domain' > 0)%nat
-        -> getD (addD cd (domain', p0)) p = Some domain
-        -> forall pre label post : string,
-            domain = (pre ++ label ++ post)%string ->
-            ValidLabel label -> (String.length label <= 63)%nat.
-    Admitted.
-
-    Lemma foo9
-      : forall cd p p0 domain domain',
-        GoodCache cd
-        -> ValidDomainName domain' /\ (String.length domain' > 0)%nat
-        -> getD (addD cd (domain', p0)) p = Some domain
-        -> ValidDomainName domain.
-    Admitted.
-
-    Lemma foo10
-      : forall cd p p0 domain domain',
-        GoodCache cd
-        -> ValidDomainName domain' /\ (String.length domain' > 0)%nat
-        -> getD (addD cd (domain', p0)) p = Some domain
-        -> gt (String.length domain) 0.
-    Admitted.
-
-    Lemma foo11
-      : forall (ce : CacheEncode) (l : DomainName) (p1 p2 : word 8),
-        getE ce l = Some (p1, p2) -> wlt (natToWord 8 191) p1.
-    Admitted.
 
 
 Definition packet_decoder
@@ -839,7 +992,7 @@ Definition packet_decoder
     rename prim_fst7 into a'; repeat destruct a' as [? a'];
       simpl in *.
     subst.
-  (* And unify with original object *) reflexivity.
+    (* And unify with original object *) reflexivity.
     decide_data_invariant.
     instantiate (1 := true).
     simpl; intros.
@@ -851,620 +1004,92 @@ Definition packet_decoder
 
     instantiate (17 := GoodCache).
     unfold cache_inv_Property; repeat split;
-      eauto using foo, foo2, foo4, foo6, foo7, foo8, foo10, foo11;
-      try solve [ eapply foo3 in H1; intuition eauto ];
-      try solve [ eapply foo9 in H2; intuition eauto ];
-      try solve [ eapply foo5 in H1; intuition eauto ].
+      eauto using cacheIndependent_add, cacheIndependent_add_2, cacheIndependent_add_4, cacheIndependent_add_6, cacheIndependent_add_7, cacheIndependent_add_8, cacheIndependent_add_10;
+      try solve [ eapply cacheIndependent_add_3 in H1; intuition eauto ];
+      try solve [ eapply cacheIndependent_add_9 in H2; intuition eauto ];
+      try solve [ eapply cacheIndependent_add_5 in H1; intuition eauto ].
     instantiate (1 := fun _ => True); exact I.
     intro; pattern idx.
     eapply Iterate_Ensemble_equiv' with (idx := idx); simpl.
     apply Build_prim_and.
     unfold cache_inv_Property; repeat split;
-      eauto using foo, foo2, foo4, foo6, foo7, foo8, foo10, foo11;
-      try solve [ eapply foo3 in H1; intuition eauto ];
-      try solve [ eapply foo9 in H2; intuition eauto ];
-      try solve [ eapply foo5 in H1; intuition eauto ].
+      eauto using cacheIndependent_add, cacheIndependent_add_2, cacheIndependent_add_4, cacheIndependent_add_6, cacheIndependent_add_7, cacheIndependent_add_8, cacheIndependent_add_10;
+      try solve [ eapply cacheIndependent_add_3 in H1; intuition eauto ];
+      try solve [ eapply cacheIndependent_add_9 in H2; intuition eauto ];
+      try solve [ eapply cacheIndependent_add_5 in H1; intuition eauto ].
     instantiate (1 := fun _ => True); exact I.
     apply Build_prim_and.
     unfold cache_inv_Property; repeat split;
-      eauto using foo, foo2, foo4, foo6, foo7, foo8, foo10, foo11;
-      try solve [ eapply foo3 in H1; intuition eauto ];
-      try solve [ eapply foo9 in H2; intuition eauto ];
-      try solve [ eapply foo5 in H1; intuition eauto ];
+      eauto using cacheIndependent_add, cacheIndependent_add_2, cacheIndependent_add_4, cacheIndependent_add_6, cacheIndependent_add_7, cacheIndependent_add_8, cacheIndependent_add_10;
+      try solve [ eapply cacheIndependent_add_3 in H1; intuition eauto ];
+      try solve [ eapply cacheIndependent_add_9 in H2; intuition eauto ];
+      try solve [ eapply cacheIndependent_add_5 in H1; intuition eauto ];
       try solve [instantiate (1 := fun _ => True); exact I].
     apply Build_prim_and.
     unfold cache_inv_Property; repeat split;
-      eauto using foo, foo2, foo4, foo6, foo7, foo8, foo10, foo11;
-      try solve [ eapply foo3 in H1; intuition eauto ];
-      try solve [ eapply foo9 in H2; intuition eauto ];
-      try solve [ eapply foo5 in H1; intuition eauto ].
+      eauto using cacheIndependent_add, cacheIndependent_add_2, cacheIndependent_add_4, cacheIndependent_add_6, cacheIndependent_add_7, cacheIndependent_add_8, cacheIndependent_add_10;
+      try solve [ eapply cacheIndependent_add_3 in H1; intuition eauto ];
+      try solve [ eapply cacheIndependent_add_9 in H2; intuition eauto ];
+      try solve [ eapply cacheIndependent_add_5 in H1; intuition eauto ].
     instantiate (1 := fun _ => True); exact I.
     apply Build_prim_and.
     unfold cache_inv_Property; repeat split;
-      eauto using foo, foo2, foo4, foo6, foo7, foo8, foo10, foo11;
-      try solve [ eapply foo3 in H1; intuition eauto ];
-      try solve [ eapply foo9 in H2; intuition eauto ];
-      try solve [ eapply foo5 in H1; intuition eauto ];
+      eauto using cacheIndependent_add, cacheIndependent_add_2, cacheIndependent_add_4, cacheIndependent_add_6, cacheIndependent_add_7, cacheIndependent_add_8, cacheIndependent_add_10;
+      try solve [ eapply cacheIndependent_add_3 in H1; intuition eauto ];
+      try solve [ eapply cacheIndependent_add_9 in H2; intuition eauto ];
+      try solve [ eapply cacheIndependent_add_5 in H1; intuition eauto ];
       try solve [instantiate (1 := fun _ => True); exact I].
     apply Build_prim_and.
     unfold cache_inv_Property; repeat split;
-      eauto using foo, foo2, foo4, foo6, foo7, foo8, foo10, foo11;
-      try solve [ eapply foo3 in H1; intuition eauto ];
-      try solve [ eapply foo9 in H2; intuition eauto ];
-      try solve [ eapply foo5 in H1; intuition eauto ].
+      eauto using cacheIndependent_add, cacheIndependent_add_2, cacheIndependent_add_4, cacheIndependent_add_6, cacheIndependent_add_7, cacheIndependent_add_8, cacheIndependent_add_10;
+      try solve [ eapply cacheIndependent_add_3 in H1; intuition eauto ];
+      try solve [ eapply cacheIndependent_add_9 in H2; intuition eauto ];
+      try solve [ eapply cacheIndependent_add_5 in H1; intuition eauto ].
     instantiate (1 := fun _ => True); exact I.
     apply Build_prim_and.
     unfold cache_inv_Property; repeat split;
-      eauto using foo, foo2, foo4, foo6, foo7, foo8, foo10, foo11;
-      try solve [ eapply foo3 in H1; intuition eauto ];
-      try solve [ eapply foo9 in H2; intuition eauto ];
-      try solve [ eapply foo5 in H1; intuition eauto ];
+      eauto using cacheIndependent_add, cacheIndependent_add_2, cacheIndependent_add_4, cacheIndependent_add_6, cacheIndependent_add_7, cacheIndependent_add_8, cacheIndependent_add_10;
+      try solve [ eapply cacheIndependent_add_3 in H1; intuition eauto ];
+      try solve [ eapply cacheIndependent_add_9 in H2; intuition eauto ];
+      try solve [ eapply cacheIndependent_add_5 in H1; intuition eauto ];
       try solve [instantiate (1 := fun _ => True); exact I].
     apply Build_prim_and.
     unfold cache_inv_Property; repeat split;
-      eauto using foo, foo2, foo4, foo6, foo7, foo8, foo10, foo11;
-      try solve [ eapply foo3 in H1; intuition eauto ];
-      try solve [ eapply foo9 in H2; intuition eauto ];
-      try solve [ eapply foo5 in H1; intuition eauto ];
+      eauto using cacheIndependent_add, cacheIndependent_add_2, cacheIndependent_add_4, cacheIndependent_add_6, cacheIndependent_add_7, cacheIndependent_add_8, cacheIndependent_add_10;
+      try solve [ eapply cacheIndependent_add_3 in H1; intuition eauto ];
+      try solve [ eapply cacheIndependent_add_9 in H2; intuition eauto ];
+      try solve [ eapply cacheIndependent_add_5 in H1; intuition eauto ];
       try solve [instantiate (1 := fun _ => True); exact I].
     apply Build_prim_and.
     unfold cache_inv_Property; repeat split;
-      eauto using foo, foo2, foo4, foo6, foo7, foo8, foo10, foo11;
-      try solve [ eapply foo3 in H1; intuition eauto ];
-      try solve [ eapply foo9 in H2; intuition eauto ];
-      try solve [ eapply foo5 in H1; intuition eauto ];
+      eauto using cacheIndependent_add, cacheIndependent_add_2, cacheIndependent_add_4, cacheIndependent_add_6, cacheIndependent_add_7, cacheIndependent_add_8, cacheIndependent_add_10;
+      try solve [ eapply cacheIndependent_add_3 in H1; intuition eauto ];
+      try solve [ eapply cacheIndependent_add_9 in H2; intuition eauto ];
+      try solve [ eapply cacheIndependent_add_5 in H1; intuition eauto ];
       try solve [instantiate (1 := fun _ => True); exact I].
     apply Build_prim_and.
     unfold cache_inv_Property; repeat split;
-      eauto using foo, foo2, foo4, foo6, foo7, foo8, foo10, foo11;
-      try solve [ eapply foo3 in H1; intuition eauto ];
-      try solve [ eapply foo9 in H2; intuition eauto ];
-      try solve [ eapply foo5 in H1; intuition eauto ];
+      eauto using cacheIndependent_add, cacheIndependent_add_2, cacheIndependent_add_4, cacheIndependent_add_6, cacheIndependent_add_7, cacheIndependent_add_8, cacheIndependent_add_10;
+      try solve [ eapply cacheIndependent_add_3 in H1; intuition eauto ];
+      try solve [ eapply cacheIndependent_add_9 in H2; intuition eauto ];
+      try solve [ eapply cacheIndependent_add_5 in H1; intuition eauto ];
       try solve [instantiate (1 := fun _ => True); exact I].
     apply Build_prim_and.
     unfold cache_inv_Property; repeat split;
-      eauto using foo, foo2, foo4, foo6, foo7, foo8, foo10, foo11;
-      try solve [ eapply foo3 in H1; intuition eauto ];
-      try solve [ eapply foo9 in H2; intuition eauto ];
-      try solve [ eapply foo5 in H1; intuition eauto ];
+      eauto using cacheIndependent_add, cacheIndependent_add_2, cacheIndependent_add_4, cacheIndependent_add_6, cacheIndependent_add_7, cacheIndependent_add_8, cacheIndependent_add_10;
+      try solve [ eapply cacheIndependent_add_3 in H1; intuition eauto ];
+      try solve [ eapply cacheIndependent_add_9 in H2; intuition eauto ];
+      try solve [ eapply cacheIndependent_add_5 in H1; intuition eauto ];
       try solve [instantiate (1 := fun _ => True); exact I].
     exact I.
     try solve [instantiate (1 := fun _ => True); exact I].
     try solve [instantiate (1 := fun _ => True); exact I].
-    Grab Existential Variables.
-    admit.
-    apply Peano_dec.eq_nat_dec.
-    apply Peano_dec.eq_nat_dec.
-    apply Peano_dec.eq_nat_dec.
-    apply weq.
-    apply weq.
-    apply weq.
-    apply weq.
-    apply weq.
-    (* Still need decideable equality lemmas for: lists of resource *)
   Defined.
 
+  Print Assumptions packet_decoder.
+  
   Definition packetDecoderImpl := Eval simpl in (projT1 packet_decoder).
 
   Print packetDecoderImpl.
-
-  (*     intros; simpl. *)
-(*     4: decode_step. *)
-(*     2: decode_step. *)
-
-(*     simpl. *)
-
-
-
-
-
-(*     repeat decode_step. *)
-
-(*     decode_step. *)
-(*     decode_step. *)
-(*     decode_step. *)
-(*     decode_step. *)
-(*     eapply String_decode_correct. *)
-(*     decode_step. *)
-(*     decode_step. *)
-(*     intros; eapply encode_decode_correct_finish. *)
-(*     build_fully_determined_type. *)
-(*     decide_data_invariant. *)
-(*     decode_step. *)
-(*     intros; instantiate (1 := fun _ _ => True). *)
-(*     decode_step. *)
-(*     decode_step. *)
-(*     decode_step. *)
-(*     decode_step. *)
-(*     decode_step. *)
-(*     decode_step. *)
-(*     decode_step. *)
-(*     eapply String_decode_correct. *)
-(*     decode_step. *)
-(*     decode_step. *)
-(*     intros; eapply encode_decode_correct_finish. *)
-(*     build_fully_determined_type. *)
-(*     decide_data_invariant. *)
-(*     decode_step. *)
-(*     intros; instantiate (1 := fun _ _ => True). *)
-(*     decode_step. *)
-(*     decode_step. *)
-
-
-(*     intros; instantiate (1 := fun _ _ => True). *)
-
-(*     solve_data_inv. *)
-(* let H' := fresh in *)
-(*   let data := fresh in *)
-(*   intros data H'; *)
-(*   repeat destruct H'; *)
-(*   match goal with *)
-(*   | H : ?P data |- ?P_inv' => *)
-(*     is_evar P; *)
-(*     let P_inv' := (eval pattern data in P_inv') in *)
-(*     let P_inv := match P_inv' with ?P_inv data => P_inv end in *)
-(*     let new_P_T := type of P in *)
-(*     makeEvar new_P_T *)
-(*              ltac:(fun new_P => *)
-(*                      unify P (fun data => new_P data /\ P_inv data)); apply (Logic.proj2 H) *)
-(*   end. *)
-
-(*     shelve_inv. *)
-
-(*     build_fully_determined_type. *)
-(*     unfold GetAttribute, GetAttributeRaw in *; *)
-(*       simpl in *; intros; intuition. *)
-(*     subst. *)
-(*     repeat *)
-(*         first [ eapply decides_and *)
-(*           | eapply decides_assumption; eassumption *)
-(*           | apply decides_eq_refl *)
-(*           | solve [eauto with decide_data_invariant_db] *)
-(*           | eapply decides_dec_eq; auto using Peano_dec.eq_nat_dec, weq ]. *)
-(*     first [ eapply decides_and *)
-(*           | eapply decides_assumption; eassumption *)
-(*           | apply decides_eq_refl *)
-(*           | solve [eauto with decide_data_invariant_db] *)
-(*           | eapply decides_dec_eq; auto using Peano_dec.eq_nat_dec, weq ]. *)
-(*         first [ eapply decides_and *)
-(*           | eapply decides_assumption; eassumption *)
-(*           | solve [eauto with decide_data_invariant_db] *)
-(*           | eapply decides_dec_eq; auto using Peano_dec.eq_nat_dec, weq ]. *)
-(*                 first [ eapply decides_and *)
-(*           | eapply decides_assumption; eassumption *)
-(*           | apply decides_eq_refl *)
-(*           | solve [eauto with decide_data_invariant_db] *)
-(*           | eapply decides_dec_eq; auto using Peano_dec.eq_nat_dec, weq ]. *)
-(*         first [ eapply decides_and *)
-(*           | eapply decides_assumption; eassumption *)
-(*           | apply decides_eq_refl *)
-(*           | solve [eauto with decide_data_invariant_db] *)
-(*           | eapply decides_dec_eq; auto using Peano_dec.eq_nat_dec, weq ]. *)
-(*         first [ eapply decides_and *)
-(*           | eapply decides_assumption; eassumption *)
-(*           | apply decides_eq_refl *)
-(*           | solve [eauto with decide_data_invariant_db] *)
-(*           | eapply decides_dec_eq; auto using Peano_dec.eq_nat_dec, weq ]. *)
-(*         eapply decides_eq_refl. *)
-(*         eapply decides_eq_refl. *)
-(*         eapply decides_eq_refl. *)
-(*     eapply decides_and *)
-(*     decode_step. *)
-
-
-(*     apply Build_prim_and. *)
-(*     repeat decode_step. *)
-
-
-(*   (* Processes the goal by either: *) *)
-(*   match goal with *)
-(*   (* A) decomposing one of the parser combinators, *) *)
-(*   | |- _ => apply_compose *)
-(*   (* B) applying one of the rules for a base type  *) *)
-(*   | H : cache_inv_Property _ _ *)
-(*     |- appcontext [encode_decode_correct_f _ _ _ _ encode_word_Spec _ _] => *)
-(*     intros; revert H; eapply Word_decode_correct *)
-(*   | |- appcontext [encode_decode_correct_f _ _ _ _ encode_word_Spec _ _] => *)
-(*     eapply Word_decode_correct *)
-(*   | |- appcontext [encode_list_Spec] => *)
-(*     intros; eapply FixList_decode_correct *)
-(*   | |- appcontext [encode_decode_correct_f _ _ _ _ (encode_nat_Spec _) _ _] => *)
-(*     eapply Nat_decode_correct *)
-(*   | |- appcontext [encode_decode_correct_f _ _ _ _ (encode_enum_Spec _) _ _] => *)
-(*     eapply Enum_decode_correct *)
-(*   (* C) Discharging a side condition of one of the base rules *) *)
-(*   | |- NoDupVector _ => Discharge_NoDupVector *)
-(*     intros; apply Vector_predicate_rest_True *)
-(*   | _ => solve [solve_data_inv] *)
-(*   (* D) Solving the goal once all the byte string has been parsed *) *)
-(*   | _ =>  solve [simpl; intros; *)
-(*                  eapply encode_decode_correct_finish; *)
-(*                  [ build_fully_determined_type *)
-(*                  | decide_data_invariant ] ] *)
-(*   end. *)
-
-(*     decode_step. *)
-
-
-(*     apply Build_prim_and. *)
-(*     repeat decode_step. *)
-
-
-
-
-(*     build_decoder. *)
-(*     apply Build_prim_and. *)
-(*     build_decoder. *)
-(*     apply Build_prim_and. *)
-(*     { *)
-(*       build_decoder. *)
-(*       build_decoder. *)
-(*       solve_data_inv. *)
-(*       build_decoder. *)
-(*       build_decoder. *)
-(*       solve_data_inv. *)
-(*       build_decoder. *)
-(*       build_decoder. *)
-(*       solve_data_inv. *)
-(*       build_decoder. *)
-(*       build_decoder. *)
-(*       solve_data_inv. *)
-(*       build_decoder. *)
-(*       build_decoder. *)
-(*       solve_data_inv. *)
-(*       build_decoder. *)
-(*       build_decoder. *)
-(*       solve_data_inv. *)
-(*       build_decoder. *)
-(*       build_decoder. *)
-(*       solve_data_inv. *)
-(*       unfold encode_decode_correct_f; intuition eauto. *)
-(*       destruct data as [? [? [? [? [? [? [? [ ] ] ] ] ] ] ] ]. *)
-(*       unfold GetAttribute, GetAttributeRaw in *. *)
-(*       subst; simpl. *)
-(*       computes_to_inv; injections. *)
-(*       eexists; intuition eauto; simpl. *)
-(*       match goal with *)
-(*         |- ?f ?a ?b ?c = ?P => *)
-(*         let P' := (eval pattern a, b, c in P) in *)
-(*         let f' := match P' with ?f a b c => f end in *)
-(*       unify f f'; reflexivity *)
-(*       end. *)
-(*       injections; eauto. *)
-(*       eexists _; eexists _. *)
-(*     intuition eauto. *)
-(*     injections; eauto. *)
-(*     injections. *)
-(*     solve_predicate. *)
-(*     injections; eauto. *)
-(*     injections; eauto. *)
-(*     injections; eauto. *)
-(*     injections; eauto. *)
-(*     injections; eauto. *)
-(*     injections; eauto. *)
-(*     injections; eauto. *)
-(*     injections; eauto. *)
-(*     injections; eauto. *)
-(*     injections; eauto. *)
-(*     injections; eauto. *)
-(*     injections; eauto. *)
-(*     } *)
-(*     apply Build_prim_and. *)
-(*     { *)
-(*       build_decoder. *)
-(*       build_decoder. *)
-(*       solve_data_inv. *)
-(*       build_decoder. *)
-(*       build_decoder. *)
-(*       solve_data_inv. *)
-(*       build_decoder. *)
-(*       build_decoder. *)
-(*       revert H21; build_decoder. *)
-(*       shelve_inv. *)
-(*       unfold encode_decode_correct_f; intuition eauto. *)
-(*       destruct data as [? [? [? [ ] ] ] ]. *)
-(*       unfold GetAttribute, GetAttributeRaw in *. *)
-(*       subst; simpl. *)
-(*       computes_to_inv; injections. *)
-(*       eexists; intuition eauto; simpl. *)
-(*       match goal with *)
-(*         |- ?f ?a ?b ?c = ?P => *)
-(*         let P' := (eval pattern a, b, c in P) in *)
-(*         let f' := match P' with ?f a b c => f end in *)
-(*         unify f f'; reflexivity *)
-(*       end. *)
-(*       simpl in H25; injections; eauto. *)
-(*       eexists _; eexists _. *)
-(*       intuition eauto. *)
-(*       injections; eauto. *)
-(*       injections. *)
-(*       solve_predicate. *)
-(*       injections; eauto. *)
-(*       injections; eauto. *)
-(*       injections; eauto. *)
-(*       injections; eauto. *)
-(*       injections; eauto. *)
-(*     } *)
-(*     apply Build_prim_and. *)
-(*     build_decoder. *)
-(*     apply Build_prim_and. *)
-(*     { *)
-(*       build_decoder. *)
-(*       build_decoder. *)
-(*       solve_data_inv. *)
-(*       build_decoder. *)
-(*       build_decoder. *)
-(*       solve_data_inv. *)
-(*       unfold encode_decode_correct_f; intuition eauto. *)
-(*       destruct data as [? [? [ ] ] ]. *)
-(*       unfold GetAttribute, GetAttributeRaw in *. *)
-(*       subst; simpl. *)
-(*       computes_to_inv; injections. *)
-(*       eexists; intuition eauto; simpl. *)
-(*       match goal with *)
-(*         |- ?f ?a ?b ?c = ?P => *)
-(*         let P' := (eval pattern a, b, c in P) in *)
-(*         let f' := match P' with ?f a b c => f end in *)
-(*         unify f f'; reflexivity *)
-(*       end. *)
-(*       injections; eauto. *)
-(*       eexists _; eexists _. *)
-(*       intuition eauto. *)
-(*       injections; eauto. *)
-(*       injections; solve_predicate. *)
-(*       injections; eauto. *)
-(*       injections; eauto. *)
-(*       injections; eauto. *)
-(*       injections; eauto. *)
-(*       injections; solve_predicate. *)
-(*     } *)
-(*     apply Build_prim_and. *)
-(*     { build_decoder. *)
-(*       build_decoder. *)
-(*       solve_data_inv. *)
-(*       build_decoder. *)
-(*       build_decoder. *)
-(*       solve_data_inv. *)
-(*       unfold encode_decode_correct_f; intuition eauto. *)
-(*       destruct data as [? [? [ ] ] ]. *)
-(*       unfold GetAttribute, GetAttributeRaw in *. *)
-(*       subst; simpl. *)
-(*       computes_to_inv; injections. *)
-(*       eexists; intuition eauto; simpl. *)
-(*       match goal with *)
-(*         |- ?f ?a ?b ?c = ?P => *)
-(*         let P' := (eval pattern a, b, c in P) in *)
-(*         let f' := match P' with ?f a b c => f end in *)
-(*         unify f f'; reflexivity *)
-(*       end. *)
-(*       injections; eauto. *)
-(*       eexists _; eexists _. *)
-(*       intuition eauto. *)
-(*       injections; eauto. *)
-(*       injections; solve_predicate. *)
-(*       injections; eauto. *)
-(*       injections; eauto. *)
-(*       injections; eauto. *)
-(*       injections; eauto. *)
-(*       injections; solve_predicate. *)
-(*       injections; solve_predicate. *)
-(*       injections; solve_predicate. *)
-(*     } *)
-(*     apply Build_prim_and. *)
-(*     { build_decoder. *)
-(*       build_decoder. *)
-(*       solve_data_inv. *)
-(*       build_decoder. *)
-(*       build_decoder. *)
-(*       solve_data_inv. *)
-(*       unfold encode_decode_correct_f; intuition eauto. *)
-(*       destruct data as [? [? [ ] ] ]. *)
-(*       unfold GetAttribute, GetAttributeRaw in *. *)
-(*       subst; simpl. *)
-(*       computes_to_inv; injections. *)
-(*       eexists; intuition eauto; simpl. *)
-(*       match goal with *)
-(*         |- ?f ?a ?b ?c = ?P => *)
-(*         let P' := (eval pattern a, b, c in P) in *)
-(*         let f' := match P' with ?f a b c => f end in *)
-(*         unify f f'; reflexivity *)
-(*       end. *)
-(*       injections; eauto. *)
-(*       eexists _; eexists _. *)
-(*       intuition eauto. *)
-(*       injections; eauto. *)
-(*       injections; solve_predicate. *)
-(*       injections; eauto. *)
-(*       injections; eauto. *)
-(*       injections; eauto. *)
-(*       injections; eauto. *)
-(*       injections; solve_predicate. *)
-(*     } *)
-(*     apply Build_prim_and. *)
-(*     build_decoder. *)
-(*     eauto. *)
-(*     shelve_inv. *)
-(*     { unfold encode_decode_correct_f; intuition eauto. *)
-(*       destruct data as [? [? [? [? [? [ ] ] ] ] ] ]. *)
-(*       unfold GetAttribute, GetAttributeRaw in *. *)
-(*       simpl in *; subst. *)
-(*       computes_to_inv; injections. *)
-(*       eexists; intuition eauto; simpl. *)
-(*       match goal with *)
-(*       |- ?f ?a ?b ?c = ?P => *)
-(*       let P' := (eval pattern a, b, c in P) in *)
-(*       let f' := match P' with ?f a b c => f end in *)
-(*       unify f f'; reflexivity *)
-(*       end. *)
-(*       injections; eauto. *)
-(*       eexists _; eexists _. *)
-(*       intuition eauto. *)
-(*       injections; eauto. *)
-(*       solve_predicate. *)
-(*       injections; eauto. *)
-(*       injections; eauto. *)
-(*       injections; eauto. *)
-(*       injections; eauto. *)
-(*       injections; eauto. *)
-(*       injections; eauto. *)
-(*       injections; eauto. *)
-(*       injections; eauto. *)
-(*       injections; eauto. *)
-(*       injections; eauto. *)
-(*     } *)
-(*     simpl; intros; intuition eauto. *)
-(*     rewrite !app_length, H20, H21, H22. *)
-(*     reflexivity. *)
-(*     generalize data H15 x H34. *)
-(*     shelve_inv. *)
-(*     generalize data H15 x H34. *)
-(*     shelve_inv. *)
-(*     generalize data H15 x H34. *)
-(*     shelve_inv. *)
-(*     generalize data H15 x H34. *)
-(*     shelve_inv. *)
-(*     simpl; intros; intuition eauto. *)
-(*     unfold encode_decode_correct_f; intuition eauto. *)
-(*     repeat destruct data. *)
-(*     repeat destruct prim_snd. *)
-(*     unfold GetAttribute, GetAttributeRaw in *. *)
-(*     computes_to_inv. *)
-(*     repeat match goal with *)
-(*              H : context [ilist2.ith2] *)
-(*              |- _ => simpl in H *)
-(*            end. *)
-(*     repeat match goal with *)
-(*              H : ?Z *)
-(*              |- _ => match Z with context [ilist2.ith2 _ _] => simpl in H *)
-(*                      end *)
-(*            end. *)
-(*     simpl. *)
-(*     destruct prim_fst7. *)
-(*     destruct prim_snd. *)
-(*     simpl in H21; simpl in H22; simpl in H23. *)
-(*     destruct prim_snd. *)
-(*     simpl in H21. *)
-(*     destruct prim_snd. *)
-(*     simpl. *)
-(*     eexists; repeat split. *)
-(*     repeat match goal with *)
-(*              H : WS _ WO = _ |- _ => *)
-(*              let H' := fresh in *)
-(*              pose proof (f_equal (@whd _) H) as H'; simpl in H'; *)
-(*                rewrite H'; clear H' H *)
-(*            end. *)
-(*     simpl in *. *)
-(*     revert H29 H27 H28; subst. *)
-(*     injection H21; intros ? ?; subst. *)
-(*     instantiate (2 := fun al ext env' => *)
-(*                          Some *)
-(*                            ({| *)
-(*       ilist.prim_fst := _; *)
-(*       ilist.prim_snd := {| *)
-(*                          ilist.prim_fst := _; *)
-(*                         ilist.prim_snd := {| *)
-(*                                           ilist.prim_fst := _; *)
-(*                                           ilist.prim_snd := {| *)
-(*                                                   ilist.prim_fst := _; *)
-(*                                                   ilist.prim_snd := {| *)
-(*                                                   ilist.prim_fst := _; *)
-(*                                                   ilist.prim_snd := {| *)
-(*                                                   ilist.prim_fst := _; *)
-(*                                                   ilist.prim_snd := {| *)
-(*                                                   ilist.prim_fst := _; *)
-(*                                                   ilist.prim_snd := {| *)
-(*                                                   ilist.prim_fst := _; *)
-(*                                                   ilist.prim_snd := {| *)
-(*                                                   ilist.prim_fst := {| *)
-(*                                                   ilist.prim_fst := _; *)
-(*                                                   ilist.prim_snd := {| *)
-(*                                                   ilist.prim_fst := _; *)
-(*                                                   ilist.prim_snd := {| *)
-(*                                                   ilist.prim_fst := _; *)
-(*                                                   ilist.prim_snd := () |} |} |}; *)
-(*                                                   ilist.prim_snd := {| *)
-(*                                                   ilist.prim_fst := firstn proj7 al; *)
-(*                                                   ilist.prim_snd := {| *)
-(*                                                   ilist.prim_fst := firstn proj8 (skipn (proj7 + proj9) al); *)
-(*                                                   ilist.prim_snd := {| *)
-(*                                                   ilist.prim_fst := firstn proj9 (skipn proj7 al); ilist.prim_snd := () |} *)
-(*                                                    |} |} |} |} |} |} |} |} |} |} |}, *)
-(*      ext, env')). *)
-(*     simpl; intros; repeat progress f_equal. *)
-(*     eauto. *)
-(*     eauto. *)
-(*     eauto. *)
-(*     subst; apply firstn_app. *)
-(*     subst; apply firstn_skipn_app. *)
-(*     subst; rewrite skipn_app. *)
-(*     apply firstn_app. *)
-(*     injections; eauto. *)
-(*     injections; eauto. *)
-(*     eexists _; eexists _; split; split; eauto. *)
-(*     injections; simpl; eauto. *)
-(*     split. *)
-(*     simpl in H21. *)
-(*     injection H21; intros; subst. *)
-(*     unfold GetAttribute, GetAttributeRaw; simpl. *)
-(*     intuition eauto. *)
-(*     solve_predicate. *)
-(*     injections; eauto. *)
-(*     eapply H18. *)
-(*     rewrite firstn_skipn_self' in H34. *)
-(*     eauto. *)
-(*     eauto. *)
-(*     rewrite H17; clear; omega. *)
-(*     eapply H18. *)
-(*     rewrite firstn_skipn_self' in H34. *)
-(*     eauto. *)
-(*     rewrite H17; clear; omega. *)
-(*     eapply H18. *)
-(*     rewrite firstn_skipn_self' in H34. *)
-(*     eauto. *)
-(*     rewrite H17; clear; omega. *)
-(*     eapply H18. *)
-(*     rewrite firstn_skipn_self' in H34. *)
-(*     eauto. *)
-(*     rewrite H17; clear; omega. *)
-(*     revert H17 H11; clear. *)
-(*     rewrite Plus.plus_assoc; intros. *)
-(*     erewrite length_firstn_skipn_app by eauto. *)
-(*     apply H11. *)
-(*     revert H17 H10; clear. *)
-(*     rewrite Plus.plus_assoc; intros. *)
-(*     erewrite length_firstn_skipn_app' by eauto. *)
-(*     apply H10. *)
-(*     revert H17 H9; clear. *)
-(*     rewrite Plus.plus_assoc; intros. *)
-(*     erewrite length_firstn_skipn_app'' by eauto. *)
-(*     apply H9. *)
-(*     apply whd_word_1_refl. *)
-(*     apply whd_word_1_refl. *)
-(*     apply whd_word_1_refl. *)
-(*     apply whd_word_1_refl. *)
-(*     apply whd_word_1_refl. *)
-(*     revert H17; clear. *)
-(*     rewrite Plus.plus_assoc; intros. *)
-(*     eapply length_firstn_skipn_app''; eauto. *)
-(*     revert H17; clear. *)
-(*     rewrite Plus.plus_assoc; intros. *)
-(*     eapply length_firstn_skipn_app'; eauto. *)
-(*     revert H17; clear. *)
-(*     rewrite Plus.plus_assoc; intros. *)
-(*     eapply length_firstn_skipn_app; eauto. *)
-(*     eapply firstn_skipn_self'. *)
-(*     rewrite H17; omega. *)
-(*     simpl in H21. *)
-(*     injection H21; intros; subst. *)
-(*     eauto. *)
-(*     repeat instantiate (1 := fun _ => True); admit. *)
-(*     Grab Existential Variables. *)
-(*     exact 0. (* Length of the Bit-Map in WKS RDATA. *) *)
-(*     apply (@Fin.F1 _). (* RDATA Type. *) *)
-(*     apply Peano_dec.eq_nat_dec. *)
-(*     intros; destruct (weqb a a') eqn:Heq; [left | right]. *)
-(*     apply weqb_sound; eauto. *)
-(*     intro; apply weqb_true_iff in H; congruence. *)
-(*   Defined. *)
 
 End DnsPacket.
